heapinsert update

HeapInsert.dfy
@@ -9,63 +9,276 @@ method HeapInsert(a: array<int>, heapsize: nat, x: int)
 	{
 	assert heapsize < a.Length;
 	assert hp(a[..], heapsize);
+	assert ph(a[..], IndexSet(0, heapsize));
+
 	//alternation
-	if heapsize == 0
+	if Guard1(heapsize)
 	{
-		a[heapsize]:=x;
+		HeapInsert1(a,heapsize,x);
+		
 	}
 	else
 	{
-		a[heapsize]:=x;
-		Heapify(a,heapsize,x);
-	}		
+		HeapInsert2(a,heapsize,x);
+		
+	}	
+	assert ph(a[..], IndexSet(0,heapsize+1));	
 	assert  hp(a[..], heapsize+1);
 	assert multiset(a[..heapsize+1]) == multiset(old(a[..heapsize])+[x]);
+	}
+
+	predicate method Guard1(heapsize:nat)
+{
+	heapsize == 0
+}
+
+	method HeapInsert1(a: array<int>, heapsize: nat, x: int)
+	requires Guard1(heapsize);
+	requires heapsize < a.Length
+	requires hp(a[..], heapsize)
+	requires ph(a[..], IndexSet(0, heapsize))
+	ensures a[heapsize]==x;
+	ensures hp(a[..], heapsize+1)
+	ensures multiset(a[..heapsize+1]) == multiset(old(a[..heapsize])+[x])
+	ensures ph(a[..], IndexSet(0, heapsize+1))
+	modifies a
+	{
+		Lemmax(a, heapsize, x);//assignemnt
+		a[heapsize]:=x;
+	}
+
+
+	lemma Lemmax (a: array<int>, heapsize: nat, x: int)
+	requires Guard1(heapsize);
+	requires heapsize < a.Length
+	requires hp(a[..], heapsize)
+	requires ph(a[..], IndexSet(0, heapsize))
+	ensures hp(a[..], heapsize+1)
+	ensures multiset(a[..heapsize+1][heapsize := x]) == multiset(old(a[..heapsize])+[x])
+	ensures ph(a[..], IndexSet(0, heapsize+1))
+	{
+	}
+
+	lemma Lemmax2 (a: array<int>, heapsize: nat, x: int)
+	requires !Guard1(heapsize);
+	requires heapsize < a.Length
+	requires hp(a[..], heapsize)
+	requires ph(a[..], IndexSet(0, heapsize))
+
+	ensures 0 < heapsize < a.Length
+	ensures multiset(a[..heapsize+1][heapsize := x]) == multiset(a[..heapsize]+[x])
+	ensures hp(a[..], heapsize)
+	ensures ph(a[..], IndexSet(0, heapsize))
+	
+	{
+	}
+
+	
+	method HeapInsert2(a: array<int>, heapsize: nat, x: int)
+	requires !Guard1(heapsize);
+	requires heapsize < a.Length
+	requires hp(a[..], heapsize)
+	requires ph(a[..], IndexSet(0, heapsize))
+	ensures hp(a[..], heapsize+1)
+	ensures multiset(a[..heapsize+1]) == multiset(old(a[..heapsize])+[x])
+	ensures ph(a[..], IndexSet(0, heapsize+1))
+	modifies a
+	{
+		Lemmax2(a, heapsize, x);//assignemnt
+		a[heapsize]:=x;
+		Heapify(a,heapsize,x);
 	}
 
 
 	method Heapify(a: array<int>,heapsize: nat, x: int)
 	requires 0 < heapsize < a.Length
-	requires  multiset(a[..heapsize+1]) == multiset(a[..heapsize]+[x])
+	requires multiset(a[..heapsize+1]) == multiset(a[..heapsize]+[x])
 	requires hp(a[..], heapsize)
+	requires a[heapsize]==x
+	requires ph(a[..], IndexSet(0, heapsize))
+
 	ensures hp(a[..], heapsize+1)
+	ensures ph(a[..], IndexSet(0, heapsize+1))
 	ensures multiset(a[..heapsize+1]) == multiset(old(a[..heapsize])+[x])
 	modifies a;
 	{
-	assert  heapsize < a.Length;
-	assert multiset(a[..heapsize+1]) == multiset(a[..heapsize]+[x]);
-	assert hp(a[..], heapsize);
-    var j:=heapsize;
-	ghost var old_seq:= a[..heapsize];
-	ghost var old_seq2:= a[..heapsize+1];
-    while (j > 0 && a[(j-1)/2] < a[j]) 
-		invariant Inv(a,heapsize,x,j,old_seq,old_seq2);
-		decreases j
-   
-    {
-		var old1:=a[(j-1)/2];
-		var old2:=a[j];
-		var old_set:= multiset(a[..heapsize+1]);
-		Swap(a, (j-1)/2, j,heapsize);
-		assert  a[(j-1)/2]==old2;
-		assert a[j]==old1;
-		assert old_set==multiset(a[..heapsize+1]);
-	  	j := (j-1)/2;
-    }
-	assert !(j > 0 && a[(j-1)/2] < a[j]);
+
+
+
+	var j,old_j,old_seq,old_seq2,i:=Init_Heapify(a,heapsize, x);
+	i,old_j,j:=Loop(j,old_j,old_seq,old_seq2,i,a,heapsize,x);
+	
+
 	assert Inv(a,heapsize,x,j,old_seq,old_seq2);
+
+
+	assert !(j > 0 && a[(j-1)/2] < a[j]);
+	assert j==0 ||  a[(j-1)/2] >= a[j];
+	
+
+	assert Inv(a,heapsize,x,j,old_seq,old_seq2);
+	
+	assert forall j:int ::
+	0<=j<heapsize+1<=a.Length && (j == 0 || (j>0 && a[(j-1)/2] >= a[j])) && Inv(a,heapsize,x,j,old_seq,old_seq2) ==> 
+	hp(a[..], j) && ph(a[..], IndexSet(0, j)) && ph(a[..], IndexSet(j, heapsize+1));
+
+
+	assert ph(a[..], IndexSet(0, j)) && ph(a[..], IndexSet(j, heapsize+1));
+	
+	assert forall j:int ::
+	0<=j<heapsize+1<=a.Length && (j == 0 || (j>0 && a[(j-1)/2] >= a[j])) && ph(a[..], IndexSet(0, j)) 
+	&& ph(a[..], IndexSet(j, heapsize+1)) && Inv(a,heapsize,x,j,old_seq,old_seq2) 
+	==> ph(a[..], IndexSet(0, heapsize+1)) && multiset(a[..heapsize+1]) == multiset(old_seq2+[x]);
+	
+	assert ph(a[..], IndexSet(0, heapsize+1));
 	assert  hp(a[..], heapsize+1);
 	assert multiset(a[..heapsize+1]) == multiset(old_seq2+[x]);
 	
 	}
 
 
-method Swap(a: array<int>, i: int, j: int,heapsize:nat)
+
+method Loop(j0:nat,old_j0:nat,old_seq:seq<int>,old_seq2:seq<int>,i0:nat,a: array<int>,heapsize: nat, x: int) returns(i:nat,old_j:nat,j:nat)
+requires j0==heapsize;
+requires old_j0 == heapsize+1;
+requires i0 == (j0-1)/2;
+requires  0< j0 <= heapsize < a.Length;
+requires Inv(a,heapsize,x,j0,old_seq,old_seq2);
+ensures j<=j0 
+ensures Inv(a,heapsize,x,j,old_seq,old_seq2) &&  (j==0 ||  a[(j-1)/2] >= a[j])
+modifies a;
+{
+
+j:=j0;
+old_j:=old_j0;
+i:=i0;
+assert j==heapsize;
+assert old_j == heapsize+1;
+assert i == (j-1)/2;
+assert  0< j <= heapsize < a.Length;
+assert Inv(a,heapsize,x,j,old_seq,old_seq2);
+
+ while (j!=0 && a[(j-1)/2] < a[j])
+		invariant Inv(a,heapsize,x,j,old_seq,old_seq2);
+		decreases j
+   
+    {
+		
+		assert Inv(a,heapsize,x,j,old_seq,old_seq2);
+		
+		assert forall j:int ::
+		0<=j<heapsize+1<=a.Length && (j > 0 && a[(j-1)/2] < a[j]) && Inv(a,heapsize,x,j,old_seq,old_seq2) ==> 
+		hp(a[..], j) && ph(a[..], IndexSet(0, j)) && ph(a[..], IndexSet(j, heapsize+1));
+
+		assert 0 < j <= heapsize && 0 < heapsize < a.Length && hp(a[..], j) && ph(a[..], IndexSet(0, j)) && ph(a[..], IndexSet(j, heapsize+1));
+				 
+		var old1:=a[(j-1)/2]; 
+		var old2:=a[j];
+		var old_set:= multiset(a[..heapsize+1]);
+		
+		  i := (j-1)/2;
+		
+		assert ph(a[..], IndexSet(0, j));
+		assert ph(a[..], IndexSet(j+1, heapsize+1));
+		assert ph(a[..], IndexSet(0, i));
+
+
+		assert ph(a[..], IndexSet(0, j));
+		assert j <= heapsize;
+		assert j == (old_j-1)/2 || (j == heapsize && old_j == heapsize+1);
+		
+
+		assert j<=heapsize;
+
+	
+		
+		assert ph(a[..], IndexSet(0, j));
+		assert ph(a[..], IndexSet(j, heapsize+1));
+		assert ph(a[..], IndexSet(j, old_j));
+		
+		Swap(a, i, j,heapsize);
+	
+		assert ph(a[..], IndexSet(0, i));
+		assert ph(a[..], IndexSet(i+1, heapsize+1));
+		assert ph(a[..], IndexSet(i, j));
+
+		assert  a[i]==old2;
+		assert a[j]==old1;
+		assert old_set == multiset(a[..heapsize+1]);
+	
+
+		  old_j := j;
+	  	   j := i;
+
+		
+		assert j == (old_j-1)/2;
+		
+		assert Inv(a,heapsize,x,j,old_seq,old_seq2);
+		assert ph(a[..], IndexSet(0, j)) && ph(a[..], IndexSet(j, heapsize+1));
+
+	}
+	assert Inv(a,heapsize,x,j,old_seq,old_seq2) &&  (j==0 ||  a[(j-1)/2] >= a[j]);
+	
+}
+
+
+method  Init_Heapify(a: array<int>,heapsize: nat, x: int) returns (j:nat,old_j:nat,old_seq:seq<int>,old_seq2:seq<int>,i:nat)
+requires 0 < heapsize < a.Length
+	requires multiset(a[..heapsize+1]) == multiset(a[..heapsize]+[x])
+	requires hp(a[..], heapsize)
+	requires a[heapsize]==x
+	requires ph(a[..], IndexSet(0, heapsize))
+	ensures j==heapsize;
+	ensures old_j == heapsize+1;
+	ensures i == (j-1)/2;
+	ensures 0<j<=heapsize<a.Length;
+
+	ensures Inv(a,heapsize,x,j,old_seq,old_seq2);
+{
+	assert  0 < heapsize < a.Length;
+	assert multiset(a[..heapsize+1]) == multiset(a[..heapsize]+[x]);
+	assert hp(a[..], heapsize);
+	assert a[heapsize]==x;
+	assert ph(a[..], IndexSet(0, heapsize));
+	
+	assert ph(a[..], IndexSet(heapsize+1, heapsize+1));
+
+     j:=heapsize;
+
+	assert ph(a[..], IndexSet(j+1, heapsize+1));
+  
+	  old_j := heapsize+1;
+	assert old_j >= j;
+
+	 old_seq:= a[..heapsize];
+	 old_seq2:= a[..heapsize+1];
+
+	assert ph(a[..], IndexSet(0, j));
+	assert ph(a[..], IndexSet(j, heapsize+1));
+	assert ph(a[..], IndexSet(j, old_j));
+
+	 i := (j-1)/2;
+	assert j == heapsize;
+	assert j == heapsize && old_j == heapsize+1;
+}
+
+
+method Swap(a: array<int>,  i: int, j: nat,heapsize:nat)
   requires 0 <= i < j <= heapsize < a.Length
   requires  a[i] < a[j]
+  requires ph(a[..], IndexSet(0, i))
+  requires ph(a[..], IndexSet(0, j))
+  requires ph(a[..], IndexSet(j+1, heapsize+1))
+
   ensures a[i] == old(a[j]);
   ensures a[j] == old(a[i]);
   ensures forall m :: heapsize < m < a.Length && m != i && m != j ==> a[m] == old(a[m]);
+  ensures a[..i] == old(a[..i])
+  ensures ph(a[..], IndexSet(0, i))
+  ensures a[i+1..j] == old(a[i+1..j])
+  ensures ph(a[..], IndexSet(i, j))
+  ensures a[j+1..] == old(a[j+1..])
+  ensures ph(a[..], IndexSet(j+1, heapsize+1))
   ensures multiset(a[..heapsize+1]) == old(multiset(a[..heapsize+1]));
   modifies a;
 {
@@ -73,18 +286,23 @@ method Swap(a: array<int>, i: int, j: int,heapsize:nat)
 }
 
 
-predicate Inv(a: array<int>,heapsize: nat, x: int , j:int ,old_seq:seq<int>,old_seq2:seq<int>)
+
+predicate Inv(a: array<int>,heapsize: nat, x: int , j:nat , old_seq:seq<int>,old_seq2:seq<int>)
 reads a;
 {
-	0 <= j <= heapsize && 
-	0 < heapsize < a.Length && 
-	 hp(a[..], j) &&
+	
+	0 < j <= heapsize && 
+	0 < heapsize < a.Length &&
+	hp(a[..], j) && 
+	
+	ph(a[..], IndexSet(0, j))&&
+	ph(a[..], IndexSet(j, heapsize+1)) &&
+	
 	multiset(a[..j+1]) == multiset(a[..j]+[x]) &&
-	multiset(a[..heapsize+1])==multiset(old_seq2) && 
+	multiset(a[..heapsize+1]) == multiset(old_seq2) && 
 	j>0 ==> AncestorIndex((j-1)/2,j) &&
 	(forall k,h :: j < h <= k <= heapsize  && (k - 1) / 2 == j && j > 0 && AncestorIndex(h, k)  ==>  a[h] >= a[k])&&				
 	a[j]==x &&
-	multiset(a[..heapsize+1]) ==multiset(old_seq+[x])
+	multiset(a[..heapsize+1]) == multiset(old_seq+[x])
 
 }
-
